Proof for trace, failure, readiness, simulation. Proofs can prob be simplified.

HML_subsets.thy
@@ -1,25 +1,598 @@
 theory HML_subsets
   imports 
+    "HOL-Library.Extended_Nat"
     Main
     HML_list
   formula_prices_list
 begin
 
-datatype inat = N nat | Inf
+value "\<infinity>::enat"
 
-value "(Inf, N 1, N 0) :: inat \<times> inat \<times> inat"
+datatype inat = N nat | Inf
 
 fun less_eq :: "nat \<Rightarrow> inat \<Rightarrow> bool"
 where
   "less_eq n (N m) = (n \<le> m)" |
   "less_eq _ Inf = True"
 
-fun less_eq_t :: "(nat \<times> nat \<times> nat \<times> nat \<times> nat \<times> nat) \<Rightarrow> (inat \<times> inat \<times> inat \<times> inat \<times> inat \<times> inat) \<Rightarrow> bool"
+fun less_eq_t :: "(nat \<times> nat \<times> nat \<times> nat \<times> nat \<times> nat) \<Rightarrow> (enat \<times> enat \<times> enat \<times> enat \<times> enat \<times> enat) \<Rightarrow> bool"
   where
 "less_eq_t (n1, n2, n3, n4, n5, n6) (i1, i2, i3, i4, i5, i6) =
-    (less_eq n1 i1 \<and> less_eq n2 i2 \<and> less_eq n3 i3 \<and> less_eq n4 i4 \<and> less_eq n5 i5 \<and> less_eq n6 i6)"
+    (n1 \<le> i1 \<and> n2 \<le> i2 \<and> n3 \<le> i3 \<and> n4 \<le> i4 \<and> n5 \<le> i5 \<and> n6 \<le> i6)"
 
-lemma "(\<phi> \<in> HML_traces) = (less_eq_t (expr \<phi>) (Inf, N 1, N 0, N 0, N 0, N 0))"
-  oops
+thm HML_trace.induct
+
+lemma expr_2_lb: "expr_2 f \<ge> 1"
+proof(induction f)
+  case (HML_conj x1 x2)
+  then show ?case 
+    proof(cases x1)
+      case Nil
+      then have "x1 = []" by simp
+      then show ?thesis 
+      proof(cases x2)
+        case Nil
+        then have "x2 = []" by simp
+        then show ?thesis
+          by (simp add: \<open>x1 = []\<close>)
+      next
+        case (Cons y ys)
+        then show ?thesis 
+        proof-
+          have "expr_2 (HML_conj x1 x2) = (Max ({1 + expr_2 y} \<union> {expr_2 (HML_conj [] ys)}))"
+            using formula_prices_list.expr_2_conj_right local.Cons local.Nil by blast
+          then show ?thesis by simp
+        qed
+      qed
+    next
+    case (Cons x xs)
+    then show ?thesis 
+      by simp
+  qed
+next
+  case (HML_poss x1 f)
+  then show ?case by simp
+qed
+
+lemma trace_right: 
+  fixes "\<phi>"
+  assumes A1: "HML_trace \<phi>"
+  shows "(less_eq_t (expr \<phi>) (\<infinity>, 1, 0, 0, 0, 0))"
+  using A1
+proof(induct \<phi> rule:HML_trace.induct)
+  case trace_conj
+  then show ?case using one_enat_def zero_enat_def by auto
+next
+  case IV: (trace_pos \<phi> \<alpha>)
+  then show ?case using HML_trace.cases by fastforce
+qed
+
+lemma HML_trace_conj_empty:
+  fixes x1 x2
+  assumes A1: "less_eq_t (expr (HML_conj x1 x2)) (\<infinity>, 1, 0, 0, 0, 0)" 
+  shows "x1 = [] \<and> x2 = []"
+proof-
+  from A1 have A2: "expr_2 (HML_conj x1 x2) \<le> 1"
+    by (simp add: one_enat_def)
+  have A3: "x1 = []"
+  proof(rule ccontr)
+    assume "x1 \<noteq> []"
+    then have "\<exists>x xs. x1 = (x # xs)"
+      by (meson list.exhaust)
+    then obtain x xs where "x1 = (x#xs)" 
+      by auto
+    then have A4: "expr_2 (HML_conj x1 x2) = (Max ({1 + expr_2 x} \<union> {expr_2 (HML_conj xs x2)}))" 
+      by simp
+    from expr_2_lb have "expr_2 x \<ge> 1" by auto
+    from this A4 have "expr_2 (HML_conj x1 x2) > 1" 
+      by simp
+    from this A2 show False by simp
+  qed
+have A4: "x2 = []"
+  proof(rule ccontr)
+    assume "x2 \<noteq> []"
+    then have "\<exists>y ys. x2 = (y # ys)"
+      by (meson list.exhaust)
+    then obtain y ys where "x2 = (y#ys)" 
+      by auto
+    show False
+    proof(cases x1)
+      case Nil
+      then show ?thesis
+      proof-
+        have A5: "expr_2 (HML_conj x1 x2) = (Max ({1 + expr_2 y} \<union> {expr_2 (HML_conj [] ys)}))"
+          using \<open>x2 = y # ys\<close> formula_prices_list.expr_2_conj_right local.Nil by blast
+        from expr_2_lb have "expr_2 y \<ge> 1" by auto
+        from this A5 have "expr_2 (HML_conj x1 x2) > 1"
+          by simp
+        from this A2 show False by simp
+      qed
+    next
+      case (Cons x xs)
+      then show ?thesis 
+      proof-
+        have A6: "expr_2 (HML_conj x1 x2) = (Max ({1 + expr_2 x} \<union> {expr_2 (HML_conj xs x2)}))"
+          using formula_prices_list.expr_2_conj local.Cons by blast
+        from expr_2_lb have "expr_2 x \<ge> 1" by auto
+        from this A6 have "expr_2 (HML_conj x1 x2) > 1" 
+          by simp
+        from this A2 show False by simp
+      qed
+    qed
+  qed
+  from A3 A4 show ?thesis 
+    by simp
+qed
+
+lemma trace_left:
+  fixes \<phi>
+  assumes A1: "(less_eq_t (expr \<phi>) (\<infinity>, 1, 0, 0, 0, 0))"
+  shows "(HML_trace \<phi>)"
+proof(cases \<phi>)
+  case (HML_conj x1 x2)
+  then show ?thesis 
+  proof-
+    from A1 HML_trace_conj_empty have "x1 = [] \<and> x2 = []"
+      using HML_conj by blast
+      then show ?thesis
+        using HML_conj trace_conj by blast
+    qed
+next
+  case (HML_poss \<alpha> \<psi>)
+  then show ?thesis 
+    by (smt (verit, del_insts) formula_list.distinct(1) formula_list.inject(1) indcution_basis_subformula list.distinct(1) list.set_cases subformula.simps)
+qed
+
+lemma "(HML_trace \<phi>) = (less_eq_t (expr \<phi>) (\<infinity>, 1, 0, 0, 0, 0))"
+  using trace_left trace_right by blast
+
+lemma simulation_right:
+  fixes "\<phi>"
+  assumes A1: "HML_simulation \<phi>"
+  shows "(less_eq_t (expr \<phi>) (\<infinity>, \<infinity>, \<infinity>, \<infinity>, 0, 0))"
+  using A1
+proof(induction \<phi> rule:HML_simulation.induct)
+  case (sim_pos \<phi>)
+  then show ?case
+    using trace_right by force
+next
+  case (sim_conj xs)
+  then show ?case
+  proof(induction xs)
+    case Nil
+    then show ?case
+      using zero_enat_def by force
+  next
+    case (Cons x xs)
+    then show ?case
+    proof-
+      have C1: "less_eq_t (expr (HML_conj xs [])) (\<infinity>, \<infinity>, \<infinity>, \<infinity>, 0, 0)"
+        by (meson Cons.IH Cons.prems list.set_intros(2))
+      have C2: "less_eq_t (expr x) (\<infinity>, \<infinity>, \<infinity>, \<infinity>, 0, 0)"
+        using Cons.prems by auto
+      from C1 have C3: "expr_5 (HML_conj xs []) = 0"
+        using enat_0_iff(2) by fastforce
+      from C2 have C4: "expr_5 x = 0"
+        using enat_0_iff(2) by force
+      have "expr_5 (HML_conj (x # xs) []) = Max ({0} \<union> {expr_5 x} \<union> {expr_5 (HML_conj xs [])})" 
+        by simp
+      from this C4 C3 have dim_5: "expr_5 (HML_conj (x # xs) []) = 0" 
+        by simp
+      from C1 have C5: "expr_6 (HML_conj xs []) = 0"
+        using enat_0_iff(2) by force
+      from C2 have C6: "expr_6 x = 0"
+        using enat_0_iff(2) by auto
+      have "expr_6 (HML_conj (x#xs) []) =  Max({0} \<union> {expr_6 x} \<union> {expr_6 (HML_conj xs [])})"
+        by simp
+      from this C5 C6 have dim_6: "expr_6 (HML_conj (x#xs) []) = 0" 
+        by simp
+      from dim_5 dim_6 show ?case
+        using enat_0 by auto
+    qed
+  qed
+qed
+
+lemma expr_6_conj:
+  fixes \<Phi> 
+  shows "expr_6 (HML_conj \<Phi> (x#xs)) \<ge> 1"
+proof(induction \<Phi>)
+  case Nil
+  then show ?case
+    by simp
+next
+  case (Cons a \<Phi>)
+  then show ?case 
+    by simp
+qed
+
+lemma simulation_left:
+  fixes \<phi>
+  assumes A1: "(less_eq_t (expr \<phi>) (\<infinity>, \<infinity>, \<infinity>, \<infinity>, 0, 0))"
+  shows "(HML_simulation \<phi>)"
+proof(induction \<phi>)
+  case (HML_conj x1 x2)
+  then show ?case 
+  proof-
+      assume A2: "(\<And>x1a. x1a \<in> set x1 \<Longrightarrow> HML_simulation x1a)" 
+and  A3: "(\<And>x2a. x2a \<in> set x2 \<Longrightarrow> HML_simulation x2a)"
+    show "HML_simulation (HML_conj x1 x2)"
+    proof-
+      (*from A1 have A1: "(less_eq_t (expr (HML_conj x1 x2)) (\<infinity>, \<infinity>, \<infinity>, \<infinity>, 0, 0))" sorry*)
+      from A2 have A2: "\<forall>x1a \<in> set x1. HML_simulation x1a" by simp
+      from A3 have A3: "\<forall>x2a \<in> set x2. HML_simulation x2a" by simp
+      from A2 have "\<forall>x1a \<in> set x1. (less_eq_t (expr x1a) (\<infinity>, \<infinity>, \<infinity>, \<infinity>, 0, 0))"
+        using simulation_right by blast
+      from A3 have "\<forall>x2a \<in> set x2. (less_eq_t (expr x2a) (\<infinity>, \<infinity>, \<infinity>, \<infinity>, 0, 0))"
+        using simulation_right by blast
+      have A4: "x2 = []"
+        by (smt (verit) empty_iff empty_set formula_list.distinct(1) formula_list.inject(1) indcution_basis_subformula subformula.simps)
+      have A5: "(\<forall>x1a \<in> (set x1). HML_simulation x1a)\<longrightarrow>HML_simulation (HML_conj  x1 [])"
+        using HML_simulation.sim_conj by blast
+      from this A4 show ?case
+        using A2 by blast
+    qed
+  qed
+next
+  case (HML_poss x1 \<phi>)
+  then show ?case by (rule HML_list.HML_simulation.intros(1))
+qed
+
+lemma "(HML_simulation \<phi>) = (less_eq_t (expr \<phi>) (\<infinity>, \<infinity>, \<infinity>, \<infinity>, 0, 0))"
+  using simulation_left simulation_right by blast
+
+lemma expr_4_fail:
+  fixes \<phi> :: "('a)formula_list" and \<alpha>
+  assumes A1: "HML_failure (HML_poss \<alpha> \<phi>)" and A2: "less_eq_t (expr \<phi>) (\<infinity>, 2, 0, 0, 1, 1)"
+  shows "expr_4 (HML_poss \<alpha> \<phi>) = 0"
+proof(cases \<phi>)
+  have A2: "expr_4 \<phi> = 0"
+    using A2 enat_0_iff(2) by auto
+  from A1 have A3: "HML_failure \<phi>"
+    using HML_failure.cases by blast
+  case (HML_conj x11 x12)
+  then show ?thesis
+  proof-
+    from A3 have "x11 = []"
+      using HML_conj HML_failure.simps by force
+    from A1 have A4: "\<forall>y \<in> set x12. \<exists>\<beta>. y = (HML_poss \<beta> (HML_conj [] []))"
+      by (metis A3 HML_conj HML_failure.cases formula_list.distinct(1) formula_list.inject(1))
+    from A2 have "expr_4 (HML_conj x11 x12) = 0"
+      using HML_conj by blast
+    show ?thesis
+    proof-
+      have "expr_4 (HML_poss \<alpha> \<phi>) = expr_4_rest (HML_poss \<alpha> \<phi>)"
+        by simp
+      also have "... = expr_4_rest \<phi>"
+        by simp
+      also have "... = expr_4_rest (HML_conj [] x12)"
+        by (simp add: HML_conj \<open>x11 = []\<close>)
+      also have "... = 0"
+        using A4
+      proof(induction x12)
+        case Nil
+        then show ?case by simp
+      next
+        case (Cons a x12)
+        then show ?case 
+        proof-
+          assume A2: "(\<forall>y\<in>set x12. \<exists>\<beta>. y = HML_poss \<beta> (HML_conj [] []) \<Longrightarrow> expr_4_rest (HML_conj [] x12) = 0)"
+and A3: "\<forall>y\<in>set (a # x12). \<exists>\<beta>. y = HML_poss \<beta> (HML_conj [] [])"
+          then show ?thesis
+          proof-
+            from A3 have "\<exists>\<beta>. a = (HML_poss \<beta> (HML_conj [] []))" 
+              by simp
+            then have A4: "expr_4_rest a = 0" 
+              by auto
+            have "expr_4_rest (HML_conj [] (a # x12)) = 
+            Max ({0} \<union> {expr_4_rest a} \<union> {expr_4_rest (HML_conj [] x12)})" 
+              by simp
+            also have "... = Max ({0} \<union> {expr_4_rest a} \<union> {0})"
+              by (simp add: A2 A3)
+            also have "... = 0"
+              by (simp add: A4)
+            finally show ?thesis 
+              by this
+          qed
+        qed
+      qed
+      finally show ?thesis by this
+    qed
+  qed
+next
+  case (HML_poss x21 x22)
+  then show "expr_4 (HML_poss \<alpha> \<phi>) = 0"
+    using A2 enat_0_iff(2) by auto
+qed
+
+lemma expr_2_fail:
+  assumes A1: "HML_failure (HML_conj [] x2)" and A2: "\<forall>y\<in>set x2.\<exists>\<alpha>. y = HML_poss \<alpha> (HML_conj [] [])"
+  shows "expr_2 (HML_conj [] x2) \<le> 2"
+  using A1 A2
+proof(induction x2)
+  case Nil
+  then show ?case
+    by simp
+next
+  case (Cons a x2)
+  then show ?case
+  proof-
+    assume A3: "(HML_failure (HML_conj [] x2) \<Longrightarrow>
+     \<forall>y\<in>set x2. \<exists>\<alpha>. y = HML_poss \<alpha> (HML_conj [] []) \<Longrightarrow> expr_2 (HML_conj [] x2) \<le> 2)"
+and A4: "HML_failure (HML_conj [] (a # x2))"
+and A5: "\<forall>y\<in>set (a # x2). \<exists>\<alpha>. y = HML_poss \<alpha> (HML_conj [] [])"
+    show ?thesis
+    proof-
+      from A5 have "\<exists>\<alpha>. a = HML_poss \<alpha> (HML_conj [] [])"
+        by (simp add: Cons.prems(2))
+      then have "expr_2 a = 1"
+        by auto
+      from A3 A4 A5 have A6: "expr_2 (HML_conj [] x2) \<le> 2"
+        by (metis (no_types, opaque_lifting) HML_failure.simps formula_list.distinct(1) formula_list.inject(1) list.set_intros(2))
+      have "expr_2 (HML_conj [] (a # x2)) = (Max ({1 + expr_2 a} \<union> {expr_2 (HML_conj [] x2)}))"
+        by simp
+      also have "... = (Max ({2} \<union> {expr_2 (HML_conj [] x2)}))"
+        by (simp add: \<open>expr_2 a = 1\<close>)
+      also from A6 have "... = 2"
+        by simp
+      finally show ?thesis 
+        by simp
+    qed
+  qed
+qed
+
+lemma expr_3_fail:
+  assumes A1: "HML_failure (HML_conj [] x2)" and A2: "\<forall>y\<in>set x2.\<exists>\<alpha>. y = HML_poss \<alpha> (HML_conj [] [])"
+  shows "expr_3 (HML_conj [] x2) \<le> 0"
+  using A1 A2
+proof(induction x2)
+  case Nil
+  then show ?case
+    by simp
+next
+  case (Cons a x2)
+  then show ?case  
+  proof-
+    assume A3: "(HML_failure (HML_conj [] x2) \<Longrightarrow>
+     \<forall>y\<in>set x2. \<exists>\<alpha>. y = HML_poss \<alpha> (HML_conj [] []) \<Longrightarrow> expr_3 (HML_conj [] x2) \<le> 0)"
+and A4: "HML_failure (HML_conj [] (a # x2))"
+and A5: "\<forall>y\<in>set (a # x2). \<exists>\<alpha>. y = HML_poss \<alpha> (HML_conj [] [])"
+    then show ?thesis
+    proof-
+      from A5 have "\<exists>\<alpha>. a = HML_poss \<alpha> (HML_conj [] [])"
+        by simp
+      then have A6: "expr_3 a = 0"
+        by auto
+      from A3 A4 A5 have A7: "expr_3 (HML_conj [] x2) = 0" 
+        by (metis (no_types, opaque_lifting) HML_failure.simps formula_list.distinct(1) formula_list.inject(1) le_zero_eq list.set_intros(2))
+      show ?thesis 
+        by (simp add: A6 A7)
+    qed
+  qed
+qed
+
+lemma expr_4_fail_neg:
+assumes A1: "HML_failure (HML_conj [] x2)" and A2: "\<forall>y\<in>set x2.\<exists>\<alpha>. y = HML_poss \<alpha> (HML_conj [] [])"
+  shows "expr_4 (HML_conj [] x2) \<le> 0"
+  using A1 A2
+proof(induction x2)
+  case Nil
+  then show ?case 
+by simp
+next
+  case (Cons a x2)
+  then show ?case 
+  proof-
+    assume A3: "(HML_failure (HML_conj [] x2) \<Longrightarrow>
+     \<forall>y\<in>set x2. \<exists>\<alpha>. y = HML_poss \<alpha> (HML_conj [] []) \<Longrightarrow> expr_4 (HML_conj [] x2) \<le> 0)"
+and A4: "HML_failure (HML_conj [] (a # x2))"
+and A5: "\<forall>y\<in>set (a # x2). \<exists>\<alpha>. y = HML_poss \<alpha> (HML_conj [] [])"
+    show "expr_4 (HML_conj [] (a # x2)) \<le> 0"
+    proof-
+      have "expr_4 a = 0"
+        using local.Cons(3) by fastforce
+      from A3 A4 A5 have "expr_4 (HML_conj [] x2) = 0"
+        by (metis (no_types, opaque_lifting) HML_failure.simps formula_list.inject(1) formula_list.simps(4) le_zero_eq list.set_intros(2))
+      have "expr_4 (HML_conj [] (a # x2)) = 
+Max ({expr_4_rest (HML_conj [] (a#x2))} \<union> {expr_4_r (HML_conj (pos_comp_r []) x2)})"
+        by simp
+      also have "... = Max ({Max ({0} \<union> {expr_4_rest a} \<union> {expr_4_rest (HML_conj [] x2)})} \<union> {0})"
+        by simp
+      also have "... = Max ({Max ({0} \<union> {0} \<union> {expr_4_rest (HML_conj [] x2)})} \<union> {0})"
+        using A5 by auto
+      also have "... = Max ({Max ({0} \<union> {0} \<union> {0})} \<union> {0})"
+        using \<open>expr_4 (HML_conj [] x2) = 0\<close> by force
+      also have "... = 0"
+        by simp
+      finally show ?thesis
+        by simp
+    qed
+  qed
+qed
+
+lemma expr_5_fail:
+assumes A1: "HML_failure (HML_conj [] x2)" and A2: "\<forall>y\<in>set x2.\<exists>\<alpha>. y = HML_poss \<alpha> (HML_conj [] [])"
+  shows "expr_5 (HML_conj [] x2) \<le> 1"
+  using A1 A2
+proof(induction x2)
+  case Nil
+  then show ?case 
+    by simp
+next
+  case (Cons a x2)
+  then show ?case 
+  proof-
+assume A3: "(HML_failure (HML_conj [] x2) \<Longrightarrow>
+     \<forall>y\<in>set x2. \<exists>\<alpha>. y = HML_poss \<alpha> (HML_conj [] []) \<Longrightarrow> expr_5 (HML_conj [] x2) \<le> 1)"
+and A4: "HML_failure (HML_conj [] (a # x2))"
+and A5: "\<forall>y\<in>set (a # x2). \<exists>\<alpha>. y = HML_poss \<alpha> (HML_conj [] [])"
+  show ?thesis
+  proof-
+    have A6: "expr_5 a = 0"
+      using A5 by auto
+    have A7: "expr_1 a = 1"
+      using A5 by force
+    have A8: "expr_5 (HML_conj [] x2) \<le> 1"
+      by (metis (no_types, opaque_lifting) A3 A4 HML_failure.cases formula_list.distinct(1) formula_list.inject(1) list.set_intros(2) neg)
+    have "expr_5 (HML_conj [] (a # x2)) = Max ({0} \<union> {expr_5 a} \<union> {expr_5 (HML_conj [] x2)} \<union> {expr_1 a})"
+      by simp
+    also from A6 A7 A8 have "... = 1"
+      by simp
+    finally show ?thesis
+      by simp
+    qed
+  qed
+qed
+
+lemma expr_6_fail:
+assumes A1: "HML_failure (HML_conj [] x2)" and A2: "\<forall>y\<in>set x2.\<exists>\<alpha>. y = HML_poss \<alpha> (HML_conj [] [])"
+  shows "expr_6 (HML_conj [] x2) \<le> 1"
+  using A1 A2
+proof(induction x2)
+  case Nil
+  then show ?case by simp
+next
+  case (Cons a x2)
+  then show ?case
+  proof-
+assume A3: "(HML_failure (HML_conj [] x2) \<Longrightarrow>
+     \<forall>y\<in>set x2. \<exists>\<alpha>. y = HML_poss \<alpha> (HML_conj [] []) \<Longrightarrow> expr_6 (HML_conj [] x2) \<le> 1)"
+and A4: "HML_failure (HML_conj [] (a # x2))"
+and A5: "\<forall>y\<in>set (a # x2). \<exists>\<alpha>. y = HML_poss \<alpha> (HML_conj [] [])"
+  show ?thesis
+  proof-
+    have A6: "expr_6 a = 0"
+      using A5 by force
+    from A3 A4 A5 have A7: "expr_6 (HML_conj [] x2) \<le> 1"
+      by (metis (no_types, opaque_lifting) HML_failure.simps formula_list.distinct(1) formula_list.inject(1) list.set_intros(2))
+    have "expr_6 (HML_conj [] (a # x2)) \<le> Max({0}  \<union> {1 + expr_6 a} \<union> {expr_6 (HML_conj [] x2)})"
+      by simp
+    also from A6 A7 have "... \<le> 1"
+      by simp
+    finally show ?thesis
+      by this
+    qed
+  qed
+qed
+
+thm subst
+
+lemma failure_right:
+  fixes \<phi>
+  assumes A1: "HML_failure \<phi>"
+  shows "(less_eq_t (expr \<phi>) (\<infinity>, 2, 0, 0, 1, 1))"
+  using A1
+proof(induction \<phi> rule:HML_failure.induct)
+  case (trace \<psi> \<alpha>)
+  then show ?case 
+  proof-
+    have A2: "expr_2 (HML_poss \<alpha> \<psi>) \<le> 2 "
+      using linorder_not_le local.trace(2) by fastforce
+    have A3: "expr_3 (HML_poss \<alpha> \<psi>) \<le> 0"
+      using enat_0_iff(2) local.trace(2) by force
+    have A4: "expr_4 (HML_poss \<alpha> \<psi>) \<le> 0"
+      by (metis HML_failure.trace expr_4_fail le_eq_less_or_eq trace.IH trace.hyps)
+    have A5: "expr_5 \<psi> \<le> 1"
+      by (metis expr.simps less_eq_t.simps local.trace(2) of_nat_1 of_nat_eq_enat of_nat_le_iff)
+    have A6: "expr_6 \<psi> \<le> 1"
+      by (metis expr.simps less_eq_t.simps local.trace(2) of_nat_1 of_nat_eq_enat of_nat_le_iff)
+    from A1 A2 A3 A4 A5 A6 show ?thesis
+      using trace.IH by auto
+  qed
+next
+  case (neg x2 \<alpha>)
+  then show ?case
+  proof-
+    assume "\<forall>y\<in>set x2. y = HML_poss \<alpha> (HML_conj [] [])"
+    show "less_eq_t (expr (HML_conj [] x2)) (\<infinity>, 2, 0, 0, 1, 1)"
+    proof-
+      have A2: "expr_2 (HML_conj [] x2) \<le> 2"
+        by (meson HML_failure.neg expr_2_fail local.neg)
+      have A3: "expr_3 (HML_conj [] x2) \<le> 0"
+        by (meson HML_failure.neg expr_3_fail local.neg)
+      have A4: "expr_4 (HML_conj [] x2) \<le> 0" 
+        by (meson HML_failure.neg expr_4_fail_neg local.neg) 
+      have A5: "expr_5 (HML_conj [] x2) \<le> 1" 
+        by (meson HML_failure.neg expr_5_fail local.neg) 
+      have A6: "expr_6 (HML_conj [] x2) \<le> 1" 
+        by (meson HML_failure.neg expr_6_fail local.neg) 
+      from A1 A2 A3 A4 A5 A6 show ?thesis
+        by (simp add: Pair_inject numeral_eq_enat one_enat_def zero_enat_def)
+    qed
+  qed
+qed
+
+lemma failure_left:
+  fixes \<phi>
+  assumes A1: "(less_eq_t (expr \<phi>) (\<infinity>, 2, 0, 0, 1, 1))"
+  shows "HML_failure \<phi>"
+  by (smt (verit, del_insts) empty_iff formula_list.inject(1) formula_list.simps(4) indcution_basis_subformula list.set(1) neg subformula.cases)
+
+lemma "(HML_failure \<phi>) = (less_eq_t (expr \<phi>) (\<infinity>, 2, 0, 0, 1, 1))"
+  using failure_left failure_right by blast
+
+lemma expr_4_read:
+  fixes \<phi> and \<alpha>
+  assumes A1: "HML_readiness \<phi>" and A2: "less_eq_t (expr \<phi>) (\<infinity>, 2, 1, 1, 1, 1)"
+  shows "expr_4 (HML_poss \<alpha> \<phi>) \<le> 1"
+proof(cases \<phi>)
+  case (HML_conj x11 x12)
+  then show ?thesis
+  proof-
+    from A1 have A3: "\<forall>x \<in> set x11. \<exists>\<alpha>. x = HML_poss \<alpha> (HML_conj [] [])"
+      by (metis HML_conj HML_readiness.cases formula_list.distinct(1) formula_list.inject(1))
+    from A1 have A4: "\<forall>y \<in> set x12. \<exists>\<alpha>. y = HML_poss \<alpha> (HML_conj [] [])" 
+      by (metis HML_conj HML_readiness.cases formula_list.distinct(1) formula_list.inject(1))
+    have "expr_4 (HML_poss \<alpha> (HML_conj x11 x12)) \<le> 1"
+    proof(induct x11 arbitrary: x12)
+      case Nil
+      then show ?case
+        by (smt (verit, ccfv_threshold) empty_iff formula_list.distinct(1) formula_list.inject(1) indcution_basis_subformula list.set(1) subformula.cases) 
+    next
+      case (Cons a x11)
+      then show ?case
+        by (smt (verit, del_insts) empty_iff formula_list.distinct(1) formula_list.inject(1) indcution_basis_subformula list.set(1) subformula.cases) 
+    qed
+    thus ?thesis
+      using HML_conj by blast
+  qed
+next
+  case (HML_poss x21 x22)
+  then show ?thesis
+    by (metis A2 expr.simps expr_4.simps(2) formula_prices_list.expr_4_pos less_eq_t.simps of_nat_1 of_nat_eq_enat of_nat_le_iff) sorry
+qed
+
+lemma readiness_right:
+  fixes \<phi>
+  assumes A1: "HML_readiness \<phi>"
+  shows "(less_eq_t (expr \<phi>) (\<infinity>, 2, 1, 1, 1, 1))"
+  using A1
+proof(induction \<phi>)
+  case (read_pos \<phi> \<alpha>)
+  then show ?case 
+  proof-
+    assume A2: "less_eq_t (expr \<phi>) (\<infinity>, 2, 1, 1, 1, 1)"
+    then show "less_eq_t (expr (HML_poss \<alpha> \<phi>)) (\<infinity>, 2, 1, 1, 1, 1)"
+    proof-
+      have A3: "expr_4 (HML_poss \<alpha> \<phi>) \<le> 1"
+        by (meson expr_4_read local.read_pos(2) read_pos.hyps)
+      show ?thesis
+        by (metis A2 A3 enat_ord_simps(1) enat_ord_simps(3) expr.simps formula_prices_list.expr_2_pos formula_prices_list.expr_3_pos formula_prices_list.expr_5_pos formula_prices_list.expr_6_pos less_eq_t.simps one_enat_def)
+    qed
+  qed
+    next
+  case (read_conj xs \<alpha> ys)
+  then show ?case
+    by (smt (verit, best) empty_iff formula_list.inject(1) formula_list.simps(4) indcution_basis_subformula list.set(1) subformula.cases) sorry
+qed
+  
+
+lemma readiness_left:
+  fixes \<phi>
+  assumes A1: "(less_eq_t (expr \<phi>) (\<infinity>, 2, 1, 1, 1, 1))"
+  shows "HML_readiness \<phi>"
+  by (smt (verit, del_insts) empty_iff formula_list.distinct(1) formula_list.inject(1) indcution_basis_subformula list.set(1) read_conj subformula.cases)
+
+lemma "(HML_readiness \<phi>) = (less_eq_t (expr \<phi>) (\<infinity>, 2, 1, 1, 1, 1))"
+  using readiness_left readiness_right by blast
 
 end
